code/experimental/P256/Hacl.Impl.LowLevel.fst
@@ -23,28 +23,114 @@ open Hacl.Spec.P256.Lemmas
 #reset-options "--z3rlimit 400"
 
 (* This code is not side channel resistant *)
-inline_for_extraction noextract
+(* inline_for_extraction noextract *)
 val eq_u64_nCT:a:uint64 -> b:uint64 -> Tot (r: bool {if uint_v a = uint_v b then r == true else r == false})
 
-(* This code is used only for proving, so the code is NOT side channel resistant *)
+(* This code is not side channel resistant *)
 let eq_u64_nCT a b =
   let open Lib.RawIntTypes in
   FStar.UInt64.(u64_to_UInt64 a =^ u64_to_UInt64 b)
 
 
 (* This code is not side channel resistant *)
-inline_for_extraction noextract
+(* inline_for_extraction noextract *)
 val eq_0_u64: a: uint64 -> Tot (r: bool {if uint_v a = 0 then r == true else r == false})
 
+(* This code is not side channel resistant *)
 let eq_0_u64 a = eq_u64_nCT a (u64 0)
 
 
-inline_for_extraction noextract
-val eq_u64_CT:a:uint64 -> b:uint64 -> Tot (r: bool {if uint_v a = uint_v b then r == true else r == false})
+val eq0_u64: a: uint64 -> Tot (r: uint64 {if uint_v a = 0 then uint_v r == pow2 64 - 1 else uint_v r == 0})
 
-let eq_u64_CT a b =
-  let r = eq_mask a b in 
-  not (eq_0_u64 r)
+let eq0_u64 a = 
+  eq_mask_lemma a (u64 0);
+  eq_mask a (u64 0)
+
+
+val eq1_u64: a: uint64 -> Tot (r: uint64 {if uint_v a = 0 then uint_v r == 0 else uint_v r == pow2 64 - 1})
+
+let eq1_u64 a = 
+  neq_mask_lemma a (u64 0);
+  neq_mask a (u64 0)
+
+
+val isZero_uint64_CT:  f: felem -> Stack uint64
+  (requires fun h -> live h f)
+  (ensures fun h0 r h1 -> modifies0 h0 h1 /\ (if as_nat h0 f = 0 then uint_v r == pow2 64 - 1 else uint_v r == 0))
+ 
+let isZero_uint64_CT f = 
+  let a0 = index f (size 0) in 
+  let a1 = index f (size 1) in 
+  let a2 = index f (size 2) in 
+  let a3 = index f (size 3) in 
+  
+  let r0 = eq_mask a0 (u64 0) in 
+  let r1 = eq_mask a1 (u64 0) in 
+  let r2 = eq_mask a2 (u64 0) in 
+  let r3 = eq_mask a3 (u64 0) in 
+  
+  let r01 = logand r0 r1 in 
+     logand_lemma r0 r1;
+  let r23 = logand r2 r3 in 
+     logand_lemma r2 r3;
+  let r = logand r01 r23 in 
+  logand_lemma r01 r23;
+      r
+
+(* This code is not side channel resistant *)
+inline_for_extraction noextract
+val isZero_uint64_nCT: f: felem -> Stack bool
+  (requires fun h -> live h f)
+  (ensures fun h0 r h1 -> modifies0 h0 h1 /\ (if as_nat h0 f = 0 then r == true else r == false))
+
+(* This code is not side channel resistant *)
+let isZero_uint64_nCT f =        
+    let f0 = index f (size 0) in  
+    let f1 = index f (size 1) in 
+    let f2 = index f (size 2) in 
+    let f3 = index f (size 3) in 
+
+    let z0_zero = eq_0_u64 f0 in 
+    let z1_zero = eq_0_u64 f1 in 
+    let z2_zero = eq_0_u64 f2 in 
+    let z3_zero = eq_0_u64 f3 in 
+  
+    z0_zero && z1_zero && z2_zero && z3_zero
+
+
+val compare_felem: a: felem -> b: felem -> Stack uint64
+  (requires fun h -> live h a /\ live h b) 
+  (ensures fun h0 r h1 -> modifies0 h0 h1 /\ (if as_nat h0 a = as_nat h0 b then uint_v r == pow2 64 - 1 else uint_v r = 0))
+
+let compare_felem a b = 
+  let a_0 = index a (size 0) in 
+  let a_1 = index a (size 1) in 
+  let a_2 = index a (size 2) in 
+  let a_3 = index a (size 3) in 
+
+  let b_0 = index b (size 0) in 
+  let b_1 = index b (size 1) in 
+  let b_2 = index b (size 2) in 
+  let b_3 = index b (size 3) in 
+
+  let r_0 = eq_mask a_0 b_0 in 
+      eq_mask_lemma a_0 b_0;
+  let r_1 = eq_mask a_1 b_1 in 
+      eq_mask_lemma a_1 b_1;
+  let r_2 = eq_mask a_2 b_2 in 
+      eq_mask_lemma a_2 b_2;
+  let r_3 = eq_mask a_3 b_3 in 
+      eq_mask_lemma a_3 b_3;
+  
+  let r01 = logand r_0 r_1 in 
+      logand_lemma r_0 r_1;
+  let r23 = logand r_2 r_3 in 
+      logand_lemma r_2 r_3;
+  
+  let r = logand r01 r23 in 
+      logand_lemma r01 r23;
+      lemma_equality (a_0, a_1, a_2, a_3) (b_0, b_1, b_2, b_3); 
+  r
 
 
 inline_for_extraction noextract
@@ -52,6 +138,7 @@ val lt_u64:a:uint64 -> b:uint64 -> Tot bool
 let lt_u64 a b =
   let open Lib.RawIntTypes in
   FStar.UInt64.(u64_to_UInt64 a <^ u64_to_UInt64 b)
+
 
 inline_for_extraction noextract
 val le_u64:a:uint64 -> b:uint64 -> Tot bool
@@ -691,59 +778,6 @@ let scalar_bit #buf_type s n =
   to_u64 ((s.(n /. 8ul) >>. (n %. 8ul)) &. u8 1)
 
 
-val isZero_uint64_CT:  f: felem -> Stack uint64
-  (requires fun h -> live h f)
-  (ensures fun h0 r h1 -> modifies0 h0 h1 /\ (if as_nat h0 f = 0 then uint_v r == pow2 64 - 1 else uint_v r == 0))
- 
-let isZero_uint64_CT f = 
-  let a0 = index f (size 0) in 
-  let a1 = index f (size 1) in 
-  let a2 = index f (size 2) in 
-  let a3 = index f (size 3) in 
-  
-  let r0 = eq_mask a0 (u64 0) in 
-  let r1 = eq_mask a1 (u64 0) in 
-  let r2 = eq_mask a2 (u64 0) in 
-  let r3 = eq_mask a3 (u64 0) in 
-  
-  let r01 = logand r0 r1 in 
-     logand_lemma r0 r1;
-  let r23 = logand r2 r3 in 
-     logand_lemma r2 r3;
-  let r = logand r01 r23 in 
-  logand_lemma r01 r23;
-      r
-
-
-inline_for_extraction noextract
-val isZero_uint64_nCT: f: felem -> Stack bool
-  (requires fun h -> live h f)
-  (ensures fun h0 r h1 -> modifies0 h0 h1 /\ (if as_nat h0 f = 0 then r == true else r == false))
-
-let isZero_uint64_nCT f =        
-    let f0 = index f (size 0) in  
-    let f1 = index f (size 1) in 
-    let f2 = index f (size 2) in 
-    let f3 = index f (size 3) in 
-
-    let z0_zero = eq_0_u64 f0 in 
-    let z1_zero = eq_0_u64 f1 in 
-    let z2_zero = eq_0_u64 f2 in 
-    let z3_zero = eq_0_u64 f3 in 
-  
-    z0_zero && z1_zero && z2_zero && z3_zero
-  
-
-
-val isZero_bool: f: felem -> Stack bool 
-  (requires fun h -> live h f) 
-  (ensures fun h0 r h1 -> modifies0 h0 h1 /\ (if as_nat h0 f = 0 then r == true else r == false))
-  
-let isZero_bool f = 
-  let r = isZero_uint64_CT f in 
-  not (eq_0_u64 r)
-
-
 val uploadOneImpl: f: felem -> Stack unit
   (requires fun h -> live h f)
   (ensures fun h0 _ h1 -> as_nat h1 f == 1 /\ modifies (loc f) h0 h1)
@@ -791,40 +825,3 @@ let copy_conditional out x mask =
 
   lemma_eq_funct_ (as_seq h1 out) (as_seq h0 out);
   lemma_eq_funct_ (as_seq h1 out) (as_seq h0 x)
-  
-
-
-val compare_felem: a: felem -> b: felem -> Stack uint64
-  (requires fun h -> live h a /\ live h b) 
-  (ensures fun h0 r h1 -> modifies0 h0 h1 /\ (if as_nat h0 a = as_nat h0 b then uint_v r == pow2 64 - 1 else uint_v r = 0))
-
-
-let compare_felem a b = 
-  let a_0 = index a (size 0) in 
-  let a_1 = index a (size 1) in 
-  let a_2 = index a (size 2) in 
-  let a_3 = index a (size 3) in 
-
-  let b_0 = index b (size 0) in 
-  let b_1 = index b (size 1) in 
-  let b_2 = index b (size 2) in 
-  let b_3 = index b (size 3) in 
-
-  let r_0 = eq_mask a_0 b_0 in 
-      eq_mask_lemma a_0 b_0;
-  let r_1 = eq_mask a_1 b_1 in 
-      eq_mask_lemma a_1 b_1;
-  let r_2 = eq_mask a_2 b_2 in 
-      eq_mask_lemma a_2 b_2;
-  let r_3 = eq_mask a_3 b_3 in 
-      eq_mask_lemma a_3 b_3;
-  
-  let r01 = logand r_0 r_1 in 
-      logand_lemma r_0 r_1;
-  let r23 = logand r_2 r_3 in 
-      logand_lemma r_2 r_3;
-  
-  let r = logand r01 r23 in 
-      logand_lemma r01 r23;
-      lemma_equality (a_0, a_1, a_2, a_3) (b_0, b_1, b_2, b_3); 
-    r
